src/Main.fst
@@ -5,7 +5,7 @@ module U32 = FStar.UInt32
 module U64 = FStar.UInt64
 module US = FStar.SizeT
 
-open SizeClass
+open FStar.Mul
 open Steel.Effect.Atomic
 open Steel.Effect
 open Steel.Array
@@ -13,7 +13,10 @@ module A = Steel.Array
 module AR = Steel.ArrayRef
 module R = Steel.Reference
 module L = Steel.SpinLock
-module SL = BlobList
+module AL = ArrayList
+
+open SizeClass
+open Utils2
 
 noeq
 type size_class =
@@ -41,8 +44,8 @@ assume val mmap_u64 (len: US.t)
       A.asel a h1 == Seq.create (US.v len) U64.zero
     )
 
-assume val mmap_blob (len: US.t)
-  : Steel (array SL.cell)
+assume val mmap_cell_status (len: US.t)
+  : Steel (array (AL.cell Slabs.status))
      emp
     (fun a -> A.varray a)
     (fun _ -> True)
@@ -56,14 +59,110 @@ assume val mmap_ptr_u32 (_:unit)
     emp
     (fun r -> R.vptr r)
 
-assume val mmap_ptr_slt (_:unit)
-  : SteelT (R.ref SL.t)
+assume val mmap_ptr_us (_:unit)
+  : SteelT (R.ref US.t)
     emp
     (fun r -> R.vptr r)
+
+
+let ind_aux pred1 pred2 pred3 r idxs : vprop =
+      AL.varraylist pred1 pred2 pred3 r
+        (US.v (fst (fst idxs)))
+        (US.v (snd (fst idxs)))
+        (US.v (snd idxs))
+
+
+val intro_ind_varraylist_nil (#a: Type) (#opened:_)
+  (pred1 pred2 pred3: a -> prop) (r: A.array (AL.cell a))
+  (r1 r2 r3: R.ref US.t)
+  : SteelGhost unit opened
+      (A.varray r `star` R.vptr r1 `star` R.vptr r2 `star` R.vptr r3)
+      (fun _ -> Slabs.ind_varraylist pred1 pred2 pred3 r r1 r2 r3)
+      (requires fun h -> A.length r == 0 /\
+        R.sel r1 h == 0sz /\
+        R.sel r2 h == 0sz /\
+        R.sel r3 h == 0sz
+      )
+      (ensures fun _ _ _ -> True)
+
+let intro_ind_varraylist_nil pred1 pred2 pred3 r r1 r2 r3 =
+  AL.intro_arraylist_nil
+    pred1 pred2 pred3
+    r
+    0sz 0sz 0sz;
+
+  let idxs = gget (R.vptr r1 `star` R.vptr r2 `star` R.vptr r3) in
+
+  assert_norm (ind_aux pred1 pred2 pred3 r ((0sz, 0sz), 0sz) ==
+          AL.varraylist pred1 pred2 pred3 r 0 0 0);
+  intro_vdep
+    (R.vptr r1 `star` R.vptr r2 `star` R.vptr r3)
+    (AL.varraylist pred1 pred2 pred3 r 0 0 0)
+    (ind_aux pred1 pred2 pred3 r)
+
+val intro_left_vprop_empty (#opened:_)
+  (slab_region: array U8.t{A.length slab_region = U32.v metadata_max * U32.v page_size})
+  (md_bm_region: array U64.t{A.length md_bm_region = U32.v metadata_max * 4})
+  (md_region: array (AL.cell Slabs.status){A.length md_region = U32.v metadata_max})
+  (r1 r2 r3: R.ref US.t)
+  : SteelGhost unit opened
+      (A.varray (split_l md_region 0sz) `star` R.vptr r1 `star` R.vptr r2 `star` R.vptr r3)
+      (fun _ -> Slabs.left_vprop 16ul slab_region md_bm_region 0ul md_region r1 r2 r3)
+      (requires fun h ->
+        R.sel r1 h == 0sz /\
+        R.sel r2 h == 0sz /\
+        R.sel r3 h == 0sz
+      )
+      (ensures fun _ _ _ -> True)
+
+let intro_left_vprop_empty slab_region md_bm_region md_region r1 r2 r3 =
+  sladmit()
+
+val intro_right_vprop_empty (#opened:_)
+  (slab_region: array U8.t{A.length slab_region = U32.v metadata_max * U32.v page_size})
+  (md_bm_region: array U64.t{A.length md_bm_region = U32.v metadata_max * 4})
+  (md_region: array (AL.cell Slabs.status){A.length md_region = U32.v metadata_max})
+  : SteelGhostT unit opened
+     (A.varray (split_r slab_region 0sz) `star`
+      A.varray (split_r md_bm_region 0sz) `star`
+      A.varray (split_r md_region 0sz))
+    (fun _ -> Slabs.right_vprop slab_region md_bm_region md_region 0ul)
+
+let intro_right_vprop_empty slab_region md_bm_region md_region =
+  sladmit()
+ // change_equal_slprop
+ //    (A.varray (A.split_r slab_region 0sz))
+ //    (A.varray (A.split_r slab_region (u32_to_sz (U32.mul v page_size))));
+ //  change_equal_slprop
+ //    (A.varray (A.split_r md_bm_region 0sz))
+ //    (A.varray (A.split_r md_bm_region (u32_to_sz (U32.mul v 4ul))));
+ //  change_equal_slprop
+ //    (A.varray (A.split_r md_region 0sz))
+ //    (A.varray (A.split_r md_region (u32_to_sz v)));
+ //  intro_vrefine
+ //    (A.varray (A.split_r slab_region (u32_to_sz (U32.mul v page_size)))) zf_u8;
+ //  intro_vrefine
+ //    (A.varray (A.split_r md_bm_region (u32_to_sz (U32.mul v 4ul)))) zf_u64;
+ //  assert_norm ((A.varray (A.split_r slab_region (u32_to_sz (U32.mul v page_size)))
+ //      `vrefine` zf_u8) `star`
+ //    (A.varray (A.split_r md_bm_region (u32_to_sz (U32.mul v 4ul)))
+ //      `vrefine` zf_u64) `star`
+ //    A.varray (A.split_r md_region (u32_to_sz v)) ==
+ //    (Slabs.right_vprop slab_region md_bm_region md_region v));
+ //  change_equal_slprop
+ //    ((A.varray (A.split_r slab_region (u32_to_sz (U32.mul v page_size)))
+ //      `vrefine` zf_u8) `star`
+ //    (A.varray (A.split_r md_bm_region (u32_to_sz (U32.mul v 4ul)))
+ //      `vrefine` zf_u64) `star`
+ //    A.varray (A.split_r md_region (u32_to_sz v)))
+ //    (Slabs.right_vprop slab_region md_bm_region md_region v);
+
 
 //TODO: move to utils
 inline_for_extraction noextract
 let u32_to_sz = Slabs.u32_to_sz
+
+open SteelVRefineDep
 
 #restart-solver
 #push-options "--z3rlimit 200 --compat_pre_typed_indexed_effects"
@@ -79,13 +178,24 @@ let init (sc:U32.t)
     = 0ul in
   let slab_region = mmap_u8 (u32_to_sz (U32.mul metadata_max page_size)) in
   let md_bm_region = mmap_u64 (u32_to_sz (U32.mul metadata_max 4ul)) in
-  let md_region = mmap_blob (u32_to_sz metadata_max) in
+  let md_region = mmap_cell_status (u32_to_sz metadata_max) in
+
+  let md_count = mmap_ptr_u32 () in
+  let ptr_partial = mmap_ptr_us () in
+  let ptr_empty = mmap_ptr_us () in
+  let ptr_full = mmap_ptr_us () in
+
   A.ghost_split slab_region 0sz;
   A.ghost_split md_bm_region 0sz;
   A.ghost_split md_region 0sz;
-  drop (A.varray (A.split_l slab_region 0sz));
-  drop (A.varray (A.split_l md_bm_region 0sz));
-  drop (A.varray (A.split_l md_region 0sz));
+
+  intro_right_vprop_empty slab_region md_bm_region md_region;
+
+(*
+  // That works
+  // drop (A.varray (A.split_l slab_region 0sz));
+  // drop (A.varray (A.split_l md_bm_region 0sz));
+  // drop (A.varray (A.split_l md_region 0sz));
   change_equal_slprop
     (A.varray (A.split_r slab_region 0sz))
     (A.varray (A.split_r slab_region (u32_to_sz (U32.mul v page_size))));
@@ -99,26 +209,142 @@ let init (sc:U32.t)
     (A.varray (A.split_r slab_region (u32_to_sz (U32.mul v page_size)))) zf_u8;
   intro_vrefine
     (A.varray (A.split_r md_bm_region (u32_to_sz (U32.mul v 4ul)))) zf_u64;
-  change_slprop_rel
+  assert_norm ((A.varray (A.split_r slab_region (u32_to_sz (U32.mul v page_size)))
+      `vrefine` zf_u8) `star`
+    (A.varray (A.split_r md_bm_region (u32_to_sz (U32.mul v 4ul)))
+      `vrefine` zf_u64) `star`
+    A.varray (A.split_r md_region (u32_to_sz v)) ==
+    (Slabs.right_vprop slab_region md_bm_region md_region v));
+  change_equal_slprop
     ((A.varray (A.split_r slab_region (u32_to_sz (U32.mul v page_size)))
       `vrefine` zf_u8) `star`
     (A.varray (A.split_r md_bm_region (u32_to_sz (U32.mul v 4ul)))
       `vrefine` zf_u64) `star`
     A.varray (A.split_r md_region (u32_to_sz v)))
-    (Slabs.vp_aux slab_region md_bm_region md_region v)
-    (fun x y -> x == y)
-    (fun _ -> admit ());
-  let md_count = mmap_ptr_u32 () in
+    (Slabs.right_vprop slab_region md_bm_region md_region v);
+*)
+
+  R.write ptr_partial 0sz;
+  R.write ptr_empty 0sz;
+  R.write ptr_full 0sz;
+
+  intro_left_vprop_empty slab_region md_bm_region md_region ptr_empty ptr_partial ptr_full;
+
+  // intro_ind_varraylist_nil Slabs.pred1 Slabs.pred2 Slabs.pred3
+  //   (A.split_l md_region 0sz)
+  //   ptr_partial ptr_empty ptr_full;
+
+  // // AL.intro_arraylist_nil
+  // //   Slabs.pred1 Slabs.pred2 Slabs.pred3
+  // //   (A.split_l md_region 0sz)
+  // //   0sz 0sz 0sz;
+
+  // // intro_vdep
+  // //   (R.vptr ptr_partial `star` R.vptr ptr_empty `star` R.vptr ptr_full)
+  // //   (AL.varraylist Slabs.pred1 Slabs.pred2 Slabs.pred3 (A.split_l md_region 0sz) 0 0 0)
+  // //   (fun (idxs: (US.t & US.t) & US.t) ->
+  // //     AL.varraylist Slabs.pred1 Slabs.pred2 Slabs.pred3 (A.split_l md_region 0sz)
+  // //       (US.v (fst (fst idxs)))
+  // //       (US.v (snd (fst idxs)))
+  // //       (US.v (snd idxs))
+  // //   );
+
+  // SteelStarSeqUtils.starseq_intro_empty #_
+  //     #(pos:U32.t{U32.v pos < U32.v 0ul})
+  //     #(Slabs.t 16ul)
+  //     (Slabs.f 16ul slab_region md_bm_region 0ul (Slabs.dataify Seq.empty))
+  //     (Slabs.f_lemma 16ul slab_region md_bm_region 0ul (Slabs.dataify Seq.empty));
+
+  // intro_vdep
+  //   (ind_varraylist pred1 pred2 pred3
+  //     (A.split_l md_region 0sz)
+  //     ptr_partial ptr_empty ptr_full)
+
+  R.write md_count 0ul;
+  SteelVRefineDep.intro_vrefinedep
+    (R.vptr md_count)
+    (fun x -> U32.v x <= U32.v metadata_max == true)
+    (size_class_vprop_aux 16ul slab_region md_bm_region md_region ptr_empty ptr_partial ptr_full)
+    (Slabs.left_vprop 16ul slab_region md_bm_region 0ul md_region
+         ptr_empty ptr_partial ptr_full `star`
+       // right part
+       Slabs.right_vprop slab_region md_bm_region md_region 0ul);
+
+
+  let scs = {
+    size = 16ul;
+    partial_slabs = ptr_partial;
+    empty_slabs = ptr_empty;
+    full_slabs = ptr_full;
+    slab_region = slab_region;
+    md_bm_region = md_bm_region;
+    md_region = md_region;
+    md_count = md_count;
+  } in
+
+
+  let open FStar.Tactics in
+  assert (
+    size_class_vprop scs ==
+    SteelVRefineDep.vrefinedep
+      (R.vptr scs.md_count)
+      (fun x -> U32.v x <= U32.v metadata_max == true)
+      (size_class_vprop_aux scs.size scs.slab_region scs.md_bm_region scs.md_region scs.empty_slabs scs.partial_slabs scs.full_slabs)
+
+      // (fun v ->
+      //   // left part
+      //   Slabs.left_vprop scs.size scs.slab_region scs.md_bm_region v scs.md_region
+      //    scs.empty_slabs scs.partial_slabs scs.full_slabs `star`
+      //   // right part
+      //   Slabs.right_vprop scs.slab_region scs.md_bm_region scs.md_region v)
+     ) by (norm [delta_only [`%size_class_vprop]]);
+
+  // vrefinedep_ext (R.vptr scs.md_count) (R.vptr md_count)
+  //     (fun x -> U32.v x <= U32.v metadata_max == true)
+  //     (size_class_vprop_aux scs.size scs.slab_region scs.md_bm_region scs.md_region scs.empty_slabs scs.partial_slabs scs.full_slabs)
+  //     (size_class_vprop_aux 16ul slab_region md_bm_region md_region ptr_empty ptr_partial ptr_full);
+
+  change_equal_slprop
+    (SteelVRefineDep.vrefinedep
+      (R.vptr md_count)
+      (fun x -> U32.v x <= U32.v metadata_max == true)
+      (size_class_vprop_aux 16ul slab_region md_bm_region md_region ptr_empty ptr_partial ptr_full))
+     (size_class_vprop scs);
+
+
+     //  (fun v ->
+     //    // left part
+     //    Slabs.left_vprop scs.size scs.slab_region scs.md_bm_region v scs.md_region
+     //     scs.empty_slabs scs.partial_slabs scs.full_slabs `star`
+     //    // right part
+     //    Slabs.right_vprop scs.slab_region scs.md_bm_region scs.md_region v)
+     // (fun v ->
+     //    // left part
+     //    Slabs.left_vprop 16ul slab_region md_bm_region v md_region
+     //     ptr_empty ptr_partial ptr_full `star`
+     //    // right part
+     //    Slabs.right_vprop slab_region md_bm_region md_region v);
+
+  drop (A.varray (A.split_l slab_region 0sz));
+  drop (A.varray (A.split_l md_bm_region 0sz));
+
+  return scs
+
+
+(*
+
+
+  return scs
+
+
+
   R.write md_count v;
   SteelVRefineDep.intro_vrefinedep
     (R.vptr md_count)
     (fun x -> U32.v x <= U32.v metadata_max == true)
-    (fun v -> Slabs.vp_aux slab_region md_bm_region md_region v)
-    (Slabs.vp_aux slab_region md_bm_region md_region v);
+    (fun v -> Slabs.right_vprop slab_region md_bm_region md_region v)
+    (Slabs.right_vprop slab_region md_bm_region md_region v);
 
-  let ptr_partial = mmap_ptr_slt () in
-  let ptr_empty = mmap_ptr_slt () in
-  let ptr_full = mmap_ptr_slt () in
 
   R.write ptr_partial SL.null_t;
   R.write ptr_empty SL.null_t;
@@ -152,11 +378,11 @@ let init (sc:U32.t)
     (R.vptr md_count)
     //TODO: hideous coercion
     (fun x -> U32.v x <= U32.v metadata_max == true)
-    (fun v -> Slabs.vp_aux slab_region md_bm_region md_region v))
+    (fun v -> Slabs.right_vprop slab_region md_bm_region md_region v))
   (size_class_vprop scs);
 
   return scs
-
+*)
 
 assume
 val size_class16 : size_class
